Tweaks

src/graph_theory/to_mathlib.lean
@@ -10,7 +10,7 @@ let f : V → quotient s := quotient.mk,
 in setoid.ker (g ∘ f)
 
 def setoid.comp.iso {V : Type} {s : setoid V} {t : setoid (quotient s)} :
-    quotient (setoid.comp s t) ≃ quotient t :=
+    quotient (s.comp t) ≃ quotient t :=
 by {
     let f : V -> quotient s := quotient.mk,
     let g : quotient s -> quotient t := quotient.mk',
@@ -20,20 +20,20 @@ by {
     have p₂ : ∀ {a b}, g a = g b <-> t.rel a b := λ a b, quotient.eq',
     have p₃ : ∀ {a b}, h a = h b <-> (s.comp t).rel a b := λ a b, quotient.eq',
     have p₄ : ∀ {a b}, (s.comp t).rel a b <-> g (f a) = g (f b) := λ a b, setoid.ker_def,
-    have p₅ : ∀ a b, s.rel a b -> h a = h b := λ a b, by { rw [p₃,p₄,<-p₁], apply congr_arg },
+    have p₅ : ∀ a b, s.rel a b -> h a = h b := λ a b, by { rw [p₃,p₄,<-p₁], exact congr_arg g },
 
-    let ζ : quotient s -> quotient (s.comp t) := λ y, quotient.lift_on' y h p₅,
+    let ζ : quotient s -> quotient (s.comp t) := λ y, y.lift_on' h p₅,
 
     have p₆ : ∀ a b, t.rel a b -> ζ a = ζ b := λ a b, by {
-        refine quotient.induction_on' a (λ x, _),
-        refine quotient.induction_on' b (λ y, _),
+        refine a.induction_on' (λ x, _),
+        refine b.induction_on' (λ y, _),
         rw [<-p₂], change g (f x) = g (f y) -> h x = h y, rw [p₃,p₄], exact id
     },
 
     exact {
-        to_fun := λ x, quotient.lift_on' x (g ∘ f) (λ _ _, id),
-        inv_fun := λ y, quotient.lift_on' y ζ p₆,
-        left_inv := λ x, quotient.induction_on' x (λ a, rfl),
+        to_fun := λ x, x.lift_on' (g ∘ f) (λ _ _, id),
+        inv_fun := λ y, y.lift_on' (λ y, y.lift_on' h p₅) p₆,
+        left_inv := λ x, quotient.induction_on' x (λ _, rfl),
         right_inv := λ y, quotient.induction_on' y (λ a, quotient.induction_on' a (λ b, rfl)),
     }
 }
